@prefix : <https://w3id.org/bim4eepsa#> .
@prefix owl: <http://www.w3.org/2002/07/owl#> .
@prefix rdf: <http://www.w3.org/1999/02/22-rdf-syntax-ns#> .
@prefix xml: <http://www.w3.org/XML/1998/namespace> .
@prefix xsd: <http://www.w3.org/2001/XMLSchema#> .
@prefix rdfs: <http://www.w3.org/2000/01/rdf-schema#> .
@base <https://w3id.org/bim4eepsa> .

<https://w3id.org/bim4eepsa> rdf:type owl:Ontology ;
                              owl:versionIRI <https://raw.githubusercontent.com/iesnaola/eepsa/master/EEPSA_previousVersions/bim4eepsa-0.2.owl> ;
                              <http://purl.org/dc/elements/1.1/publisher> "IK4-TEKNIKER (http://www.tekniker.es)" ;
                              <http://purl.org/dc/elements/1.1/title> "BIM for EEPSA" ;
                              <http://purl.org/dc/terms/creator> """Iker Esnaola-Gonzalez <mailto:iker.esnaola@tekniker.es>
Jesús Bermúdez <mailto:jesus.bermudez@ehu.eus>"""@en ;
                              <http://purl.org/dc/terms/issued> "2017-07-10" ;
                              <http://purl.org/dc/terms/license> "This work is licensed under the Creative Commons Attribution-NonCommercial 4.0 International License. To view a copy of this license, visit http://creativecommons.org/licenses/by-nc/4.0/."@en ;
                              <http://purl.org/ontology/bibo/status> "Work in progress"@en ;
                              <http://purl.org/vocab/vann/preferredNamespacePrefix> "bim4eepsa" ;
                              rdfs:comment "Building and space-related information for the EEPSA Ontology."@en ;
                              owl:versionInfo 0.2 .

#################################################################
#    Annotation properties
#################################################################

###  http://purl.org/dc/elements/1.1/date
<http://purl.org/dc/elements/1.1/date> rdf:type owl:AnnotationProperty .


###  http://purl.org/dc/elements/1.1/description
<http://purl.org/dc/elements/1.1/description> rdf:type owl:AnnotationProperty .


###  http://purl.org/dc/elements/1.1/publisher
<http://purl.org/dc/elements/1.1/publisher> rdf:type owl:AnnotationProperty .


###  http://purl.org/dc/elements/1.1/title
<http://purl.org/dc/elements/1.1/title> rdf:type owl:AnnotationProperty .


###  http://purl.org/dc/terms/creator
<http://purl.org/dc/terms/creator> rdf:type owl:AnnotationProperty .


###  http://purl.org/dc/terms/issued
<http://purl.org/dc/terms/issued> rdf:type owl:AnnotationProperty .


###  http://purl.org/dc/terms/license
<http://purl.org/dc/terms/license> rdf:type owl:AnnotationProperty .


###  http://purl.org/ontology/bibo/status
<http://purl.org/ontology/bibo/status> rdf:type owl:AnnotationProperty .


###  http://purl.org/vocab/vann/preferredNamespacePrefix
<http://purl.org/vocab/vann/preferredNamespacePrefix> rdf:type owl:AnnotationProperty .


###  http://www.w3.org/2002/07/owl#versionInfo
owl:versionInfo rdf:type owl:AnnotationProperty .


###  http://www.w3.org/2003/01/geo/wgs84_pos#alt
<http://www.w3.org/2003/01/geo/wgs84_pos#alt> rdf:type owl:AnnotationProperty ;
                                              rdfs:comment """The WGS84 altitude of a SpatialThing (decimal meters 
above the local reference ellipsoid).""" ;
                                              rdfs:label "altitude" ;
                                              rdfs:domain <http://www.w3.org/2003/01/geo/wgs84_pos#SpatialThing> .


###  http://www.w3.org/2003/01/geo/wgs84_pos#lat
<http://www.w3.org/2003/01/geo/wgs84_pos#lat> rdf:type owl:AnnotationProperty ;
                                              rdfs:comment "The WGS84 latitude of a SpatialThing (decimal degrees)." ;
                                              rdfs:label "latitude" ;
                                              rdfs:domain <http://www.w3.org/2003/01/geo/wgs84_pos#SpatialThing> .


###  http://www.w3.org/2003/01/geo/wgs84_pos#location
<http://www.w3.org/2003/01/geo/wgs84_pos#location> rdf:type owl:AnnotationProperty ;
                                                   rdfs:subPropertyOf <http://xmlns.com/foaf/0.1/based_near> ;
                                                   rdfs:range <http://www.w3.org/2003/01/geo/wgs84_pos#SpatialThing> .


###  http://www.w3.org/2003/01/geo/wgs84_pos#long
<http://www.w3.org/2003/01/geo/wgs84_pos#long> rdf:type owl:AnnotationProperty ;
                                               rdfs:comment "The WGS84 longitude of a SpatialThing (decimal degrees)." ;
                                               rdfs:label "longitude" ;
                                               rdfs:domain <http://www.w3.org/2003/01/geo/wgs84_pos#SpatialThing> .


###  http://www.w3.org/ns/prov#hadPrimarySource
<http://www.w3.org/ns/prov#hadPrimarySource> rdf:type owl:AnnotationProperty .


###  http://xmlns.com/foaf/0.1/based_near
<http://xmlns.com/foaf/0.1/based_near> rdf:type owl:AnnotationProperty .


#################################################################
#    Object Properties
#################################################################

###  http://www.w3.org/2003/01/geo/wgs84_pos#location
<http://www.w3.org/2003/01/geo/wgs84_pos#location> rdf:type owl:ObjectProperty .


###  https://w3id.org/def/saref4bldg#contains
<https://w3id.org/def/saref4bldg#contains> rdf:type owl:ObjectProperty ;
                                           owl:inverseOf <https://w3id.org/def/saref4bldg#isContainedIn> ;
                                           rdf:type owl:TransitiveProperty ;
                                           rdfs:comment "A relation between a physical space and the objects located in such space."@en ;
                                           rdfs:label "contains"@en .


###  https://w3id.org/def/saref4bldg#hasSpace
<https://w3id.org/def/saref4bldg#hasSpace> rdf:type owl:ObjectProperty ;
                                           owl:inverseOf <https://w3id.org/def/saref4bldg#isSpaceOf> ;
                                           rdf:type owl:TransitiveProperty ;
                                           rdfs:comment "Relation between a building or a building space and the spaces it can be divided into."@en ;
                                           rdfs:label "has space"@en .


###  https://w3id.org/def/saref4bldg#isContainedIn
<https://w3id.org/def/saref4bldg#isContainedIn> rdf:type owl:ObjectProperty ,
                                                         owl:TransitiveProperty ;
                                                rdfs:comment "A relation between an object and the physical space in which it is located."@en ;
                                                rdfs:label "is contained in"@en .


###  https://w3id.org/def/saref4bldg#isSpaceOf
<https://w3id.org/def/saref4bldg#isSpaceOf> rdf:type owl:ObjectProperty ,
                                                     owl:TransitiveProperty ;
                                            rdfs:comment "Relation between a building space and the building or building space it belongs to."@en ;
                                            rdfs:label "isSpaceOf"@en .


#################################################################
#    Data properties
#################################################################

###  https://w3id.org/bim4eepsa#pset_BuildingCommon_buildingID
:pset_BuildingCommon_buildingID rdf:type owl:DatatypeProperty ;
                                rdfs:range xsd:string ;
                                rdfs:comment "A unique identifier assigned to a building. A temporary identifier is initially assigned at the time of making a planning application. This temporary identifier is changed to a permanent identifier when the building is registered into a statutory buildings and properties database."@en ;
                                rdfs:label "Building ID"@en .


###  https://w3id.org/bim4eepsa#pset_BuildingCommon_constructionMethod
:pset_BuildingCommon_constructionMethod rdf:type owl:DatatypeProperty ;
                                        rdfs:range xsd:string ;
                                        rdfs:comment "The type of intervention on the building: new construction, renovation, rehabilitation, etc."@en ;
                                        rdfs:label "Construction method"@en .


###  https://w3id.org/bim4eepsa#pset_BuildingCommon_fireProtectionClass
:pset_BuildingCommon_fireProtectionClass rdf:type owl:DatatypeProperty ;
                                         rdfs:range xsd:string ;
                                         rdfs:comment "Main fire protection class for the building which is assigned from the fire protection classification table as given by the relevant national building code."@en ;
                                         rdfs:label "Fire protection class"@en .


###  https://w3id.org/bim4eepsa#pset_BuildingCommon_grossPlannedArea
:pset_BuildingCommon_grossPlannedArea rdf:type owl:DatatypeProperty ;
                                      rdfs:range xsd:double ;
                                      rdfs:comment "Total planned gross area for the building Used for programming the building."@en ;
                                      rdfs:label "Gross planned area"@en .


###  https://w3id.org/bim4eepsa#pset_BuildingCommon_netPlannedArea
:pset_BuildingCommon_netPlannedArea rdf:type owl:DatatypeProperty ;
                                    rdfs:range xsd:double ;
                                    rdfs:comment "Total planned net area for the building Used for programming the building."@en ;
                                    rdfs:label "Net planned area"@en .


###  https://w3id.org/bim4eepsa#pset_BuildingCommon_numberOfStoreys
:pset_BuildingCommon_numberOfStoreys rdf:type owl:DatatypeProperty ;
                                     rdfs:range xsd:integer ;
                                     rdfs:comment "The number of storeys within a building. Captured for those cases where the IfcBuildingStorey entity is not used. Note that if IfcBuilingStorey is asserted and the number of storeys in a building can be determined from it, then this approach should be used in preference to setting a property for the number of storeys."@en ;
                                     rdfs:label "Number of storeys"@en .


###  https://w3id.org/bim4eepsa#pset_BuildingCommon_occupancyType
:pset_BuildingCommon_occupancyType rdf:type owl:DatatypeProperty ;
                                   rdfs:range xsd:string ;
                                   rdfs:comment "Occupancy type for this object. It is defined according to the presiding national building code."@en ;
                                   rdfs:label "Occupancy type"@en .


###  https://w3id.org/bim4eepsa#pset_BuildingCommon_yearOfConstruction
:pset_BuildingCommon_yearOfConstruction rdf:type owl:DatatypeProperty ;
                                        rdfs:range xsd:integer ;
                                        rdfs:comment "Year of construction of this building, including expected year of completion."@en ;
                                        rdfs:label "Year of construction"@en .


###  https://w3id.org/bim4eepsa#pset_BuildingCommon_yearOfLastRefurbishment
:pset_BuildingCommon_yearOfLastRefurbishment rdf:type owl:DatatypeProperty ;
                                             rdfs:range xsd:integer ;
                                             rdfs:comment "Year of last major refurbishment, or reconstruction, of the building (applies to reconstruction works)."@en ;
                                             rdfs:label "Year of last refurbishment"@en .


###  https://w3id.org/bim4eepsa#pset_BuildingUse_marketCategory
:pset_BuildingUse_marketCategory rdf:type owl:DatatypeProperty ;
                                 rdfs:comment "Category of use e.g. residential, commercial, recreation etc."@en ;
                                 rdfs:label "Market category"@en .


###  https://w3id.org/bim4eepsa#pset_BuildingUse_marketSubCategory
:pset_BuildingUse_marketSubCategory rdf:type owl:DatatypeProperty ;
                                    rdfs:comment "Subset of category of use e.g. multi-family, 2 bedroom, low rise."@en ;
                                    rdfs:label "Market sub category"@en .


###  https://w3id.org/bim4eepsa#pset_BuildingUse_narrativeText
:pset_BuildingUse_narrativeText rdf:type owl:DatatypeProperty ;
                                rdfs:comment "Added information relating to the adjacent building use that is not appropriate to the general descriptive text associated with an entity through the inherited IfcRoot.Description."@en ;
                                rdfs:label "Narrative text"@en .


###  https://w3id.org/bim4eepsa#pset_BuildingUse_planningControlStatus
:pset_BuildingUse_planningControlStatus rdf:type owl:DatatypeProperty ;
                                        rdfs:comment "Label of zoning category or class, or planning control category for the site or facility."@en ;
                                        rdfs:label "Planning control status"@en .


#################################################################
#    Classes
#################################################################

###  http://www.w3.org/2003/01/geo/wgs84_pos#Point
<http://www.w3.org/2003/01/geo/wgs84_pos#Point> rdf:type owl:Class ;
                                                rdfs:subClassOf <http://www.w3.org/2003/01/geo/wgs84_pos#SpatialThing> ;
                                                rdfs:comment """ 
Uniquely identified by lat/long/alt. i.e.

spaciallyIntersects(P1, P2) :- lat(P1, LAT), long(P1, LONG), alt(P1, ALT),
  lat(P2, LAT), long(P2, LONG), alt(P2, ALT).

sameThing(P1, P2) :- type(P1, Point), type(P2, Point), spaciallyIntersects(P1, P2).
  """ ,
                                                             """A point, typically described using a coordinate system relative to Earth, such as WGS84.
  """ ;
                                                rdfs:label "point" .


###  http://www.w3.org/2003/01/geo/wgs84_pos#SpatialThing
<http://www.w3.org/2003/01/geo/wgs84_pos#SpatialThing> rdf:type owl:Class ;
                                                       rdfs:comment "Anything with spatial extent, i.e. size, shape, or position. e.g. people, places, bowling balls, as well as abstract areas like cubes."@en ,
                                                                    """Anything with spatial extent, i.e. size, shape, or position.
 e.g. people, places, bowling balls, as well as abstract areas like cubes.
""" ;
                                                       rdfs:isDefinedBy <http://www.w3.org/2003/01/geo/wgs84_pos#> ;
                                                       rdfs:label "Spatial thing"@en ,
                                                                  "SpatialThing" .


###  https://w3id.org/bim4eepsa#BuildingElement
:BuildingElement rdf:type owl:Class ;
                 rdfs:subClassOf <https://w3id.org/def/saref4bldg#PhysicalObject> ;
                 rdfs:comment "The building element comprises all elements that are primarily part of the construction of a building, i.e., its structural and space separating system."@en ;
                 rdfs:label "Building Element"@en ;
                 rdfs:seeAlso <http://ifcowl.openbimstandards.org/IFC4_ADD2#IfcBuildingElement> .


###  https://w3id.org/bim4eepsa#Door
:Door rdf:type owl:Class ;
      rdfs:subClassOf :BuildingElement ;
      rdfs:comment "Definition according to ISO 6707-1: construction for closing an opening, intended primarily for access with hinged, pivoted or sliding operation."@en ;
      rdfs:label "Door"@en ;
      rdfs:seeAlso <http://ifcowl.openbimstandards.org/IFC4_ADD2#IfcDoor> .


###  https://w3id.org/bim4eepsa#ExternalBuildingElement
:ExternalBuildingElement rdf:type owl:Class ;
                         rdfs:subClassOf :BuildingElement ;
                         rdfs:comment "A building element that is external (face the outside of the building)"@en ;
                         rdfs:label "External building element"@en .


###  https://w3id.org/bim4eepsa#ExternalDoor
:ExternalDoor rdf:type owl:Class ;
              owl:equivalentClass [ owl:intersectionOf ( :Door
                                                         :ExternalBuildingElement
                                                       ) ;
                                    rdf:type owl:Class
                                  ] ;
              rdfs:subClassOf :Door ;
              rdfs:label "External door"@en ;
              rdfs:seeAlso "A door that is external (facing the outside of the building)"@en .


###  https://w3id.org/bim4eepsa#ExternalWall
:ExternalWall rdf:type owl:Class ;
              owl:equivalentClass [ owl:intersectionOf ( :ExternalBuildingElement
                                                         :Wall
                                                       ) ;
                                    rdf:type owl:Class
                                  ] ;
              rdfs:subClassOf :Wall ;
              rdfs:label "External wall"@en ;
              rdfs:seeAlso "A wall that is external (facing the outside of the building)"@en .


###  https://w3id.org/bim4eepsa#ExternalWindow
:ExternalWindow rdf:type owl:Class ;
                owl:equivalentClass [ owl:intersectionOf ( :ExternalBuildingElement
                                                           :Window
                                                         ) ;
                                      rdf:type owl:Class
                                    ] ;
                rdfs:subClassOf :Window ;
                rdfs:comment "A window that is external (facing the outside of the building)"@en ;
                rdfs:label "External window"@en .


###  https://w3id.org/bim4eepsa#Roof
:Roof rdf:type owl:Class ;
      rdfs:subClassOf :BuildingElement ;
      rdfs:comment "Definition according to ISO 6707-1: construction enclosing the building from above."@en ;
      rdfs:label "Roof"@en ;
      rdfs:seeAlso <http://ifcowl.openbimstandards.org/IFC4_ADD2#IfcRoof> .


###  https://w3id.org/bim4eepsa#Skylight
:Skylight rdf:type owl:Class ;
          rdfs:subClassOf :BuildingElement ;
          rdfs:label "Skylight"@en ;
          rdfs:seeAlso "Skylights are light transmitting fenestration (elements filling building envelope openings) forming all, or a portion of, the roof of a building's space for daylighting purposes. (Wikipedia)"@en .


###  https://w3id.org/bim4eepsa#Wall
:Wall rdf:type owl:Class ;
      rdfs:subClassOf :BuildingElement ;
      rdfs:comment "Definition according to ISO 6707-1: vertical construction usually in masonry or in concrete which bounds or subdivides a construction works and fulfils a load bearing or retaining function."@en ;
      rdfs:label "Wall"@en ;
      rdfs:seeAlso <http://ifcowl.openbimstandards.org/IFC4_ADD2#IfcWall> .


###  https://w3id.org/bim4eepsa#WeatherStation
:WeatherStation rdf:type owl:Class ;
                rdfs:subClassOf <https://w3id.org/def/saref4bldg#Building> ;
                rdfs:comment "A weather station is a facility, either on land or sea, with instruments and equipment for measuring atmospheric conditions to provide information for weather forecasts and to study the weather and climate (Wikipedia)"@en ;
                rdfs:label <http://aemet.linkeddata.es/ontology/WeatherStation> ,
                           "Weather station"@en .


###  https://w3id.org/bim4eepsa#Window
:Window rdf:type owl:Class ;
        rdfs:subClassOf :BuildingElement ;
        rdfs:comment "Definition according to ISO 6707-1: Construction for closing a vertical or near vertical opening in a wall or pitched roof that will admit light and may admit fresh air."@en ;
        rdfs:label "Window"@en ;
        rdfs:seeAlso <http://ifcowl.openbimstandards.org/IFC4_ADD2#IfcWindow> .


###  https://w3id.org/def/saref4bldg#Building
<https://w3id.org/def/saref4bldg#Building> rdf:type owl:Class ;
                                           rdfs:subClassOf <http://www.w3.org/2003/01/geo/wgs84_pos#SpatialThing> ,
                                                           [ rdf:type owl:Restriction ;
                                                             owl:onProperty <http://www.w3.org/2003/01/geo/wgs84_pos#location> ;
                                                             owl:allValuesFrom <http://www.w3.org/2003/01/geo/wgs84_pos#SpatialThing>
                                                           ] ,
                                                           [ rdf:type owl:Restriction ;
                                                             owl:onProperty <https://w3id.org/def/saref4bldg#hasSpace> ;
                                                             owl:allValuesFrom <https://w3id.org/def/saref4bldg#BuildingSpace>
                                                           ] ,
                                                           [ rdf:type owl:Restriction ;
                                                             owl:onProperty :pset_BuildingCommon_buildingID ;
                                                             owl:allValuesFrom xsd:string
                                                           ] ,
                                                           [ rdf:type owl:Restriction ;
                                                             owl:onProperty :pset_BuildingCommon_numberOfStoreys ;
                                                             owl:allValuesFrom xsd:integer
                                                           ] ,
                                                           [ rdf:type owl:Restriction ;
                                                             owl:onProperty :pset_BuildingCommon_occupancyType ;
                                                             owl:allValuesFrom xsd:string
                                                           ] ;
                                           rdfs:comment "A building represents a structure that provides shelter for its occupants or contents and stands in one place. The building is also used to provide a basic element within the spatial structure hierarchy for the components of a building project (together with site, storey, and space)."@en ;
                                           rdfs:label "Building"@en ;
                                           rdfs:seeAlso <https://w3id.org/ifc/IFC4_ADD1#IfcBuilding> ;
                                           <http://www.w3.org/ns/prov#hadPrimarySource> <http://www.buildingsmart-tech.org/ifc/IFC4/Add1/html/schema/ifcproductextension/lexical/ifcbuilding.htm> .


###  https://w3id.org/def/saref4bldg#BuildingSpace
<https://w3id.org/def/saref4bldg#BuildingSpace> rdf:type owl:Class ;
                                                rdfs:subClassOf <http://www.w3.org/2003/01/geo/wgs84_pos#SpatialThing> ,
                                                                [ rdf:type owl:Restriction ;
                                                                  owl:onProperty <https://w3id.org/def/saref4bldg#contains> ;
                                                                  owl:allValuesFrom <https://w3id.org/def/saref4bldg#PhysicalObject>
                                                                ] ,
                                                                [ rdf:type owl:Restriction ;
                                                                  owl:onProperty <https://w3id.org/def/saref4bldg#hasSpace> ;
                                                                  owl:allValuesFrom <https://w3id.org/def/saref4bldg#BuildingSpace>
                                                                ] ,
                                                                [ rdf:type owl:Restriction ;
                                                                  owl:onProperty <https://w3id.org/def/saref4bldg#isSpaceOf> ;
                                                                  owl:allValuesFrom [ rdf:type owl:Class ;
                                                                                      owl:unionOf ( <https://w3id.org/def/saref4bldg#Building>
                                                                                                    <https://w3id.org/def/saref4bldg#BuildingSpace>
                                                                                                  )
                                                                                    ]
                                                                ] ;
                                                rdfs:comment "An entity used to define the physical spaces of the building. A building space contains devices or building objects."@en ;
                                                rdfs:label "Building space"@en .


###  https://w3id.org/def/saref4bldg#PhysicalObject
<https://w3id.org/def/saref4bldg#PhysicalObject> rdf:type owl:Class ;
                                                 rdfs:subClassOf <http://www.w3.org/2003/01/geo/wgs84_pos#SpatialThing> ,
                                                                 [ rdf:type owl:Restriction ;
                                                                   owl:onProperty <http://www.w3.org/2003/01/geo/wgs84_pos#location> ;
                                                                   owl:allValuesFrom <http://www.w3.org/2003/01/geo/wgs84_pos#SpatialThing>
                                                                 ] ,
                                                                 [ rdf:type owl:Restriction ;
                                                                   owl:onProperty <https://w3id.org/def/saref4bldg#contains> ;
                                                                   owl:allValuesFrom <https://w3id.org/def/saref4bldg#PhysicalObject>
                                                                 ] ,
                                                                 [ rdf:type owl:Restriction ;
                                                                   owl:onProperty <https://w3id.org/def/saref4bldg#isContainedIn> ;
                                                                   owl:allValuesFrom [ rdf:type owl:Class ;
                                                                                       owl:unionOf ( <https://w3id.org/def/saref4bldg#BuildingSpace>
                                                                                                     <https://w3id.org/def/saref4bldg#PhysicalObject>
                                                                                                   )
                                                                                     ]
                                                                 ] ;
                                                 rdfs:comment "Any Object that has a proper space region.  (Definition extracted from DUL ontology)"@en ;
                                                 rdfs:label "Physical object"@en .


#################################################################
#    Annotations
#################################################################

<http://www.w3.org/2003/01/geo/wgs84_pos#> <http://purl.org/dc/elements/1.1/date> "$Date: 2009/04/20 15:00:30 $" ;
                                           <http://purl.org/dc/elements/1.1/description> """A vocabulary for representing latitude, longitude and 
 altitude information in the WGS84 geodetic reference datum. 
 Version $Id: wgs84_pos.rdf,v 1.22 2009/04/20 15:00:30 timbl Exp $. See http://www.w3.org/2003/01/geo/ for more details.""" ;
                                           <http://purl.org/dc/elements/1.1/title> "WGS84 Geo Positioning: an RDF vocabulary" ;
                                           rdfs:comment """
Recent changes to this namespace:
$Log: wgs84_pos.rdf,v $
Revision 1.22  2009/04/20 15:00:30  timbl
Remove the time bits which have been deal with elsewhere eg in iCal.

Revision 1.21  2009/04/20 12:52:47  timbl
try again

Revision 1.20  2009/04/20 12:42:11  timbl
Add Event (edited ages ago and never checked in), and location (following discussion http://chatlogs.planetrdf.com/swig/2009-04-20#T12-36-09)

Revision 1.19  2009/04/20 12:36:31  timbl
Add Event (edited ages ago and never checked in), and location (following discussion http://chatlogs.planetrdf.com/swig/2009-04-20#T12-36-09)

Revision 1.18  2006/02/01 22:01:04  danbri
Clarified that lat and long are decimal degrees, and that alt is decimal metres about local reference ellipsoid

Revision 1.17  2004/02/06 17:38:12  danbri
Fixed a bad commit screwup

Revision 1.15  2003/04/19 11:24:08  danbri
Fixed the typo even more.

Revision 1.14  2003/04/19 11:16:56  danbri
fixed a typo

Revision 1.13  2003/02/19 22:27:27  connolly
relaxed domain constraints on lat/long/alt from Point to SpatialThing

Revision 1.12  2003/01/12 01:41:41  danbri
Trying local copy of XSLT doc.

Revision 1.11  2003/01/12 01:20:18  danbri
added a link to morten's xslt rdfs viewer.

Revision 1.10  2003/01/11 18:56:49  danbri
Removed datatype range from lat and long properties, since they would
have required each occurance of the property to mention the datatype.

Revision 1.9  2003/01/11 11:41:31  danbri
Another typo; repaired rdfs:Property to rdf:Property x4

Revision 1.8  2003/01/11 11:05:02  danbri
Added an rdfs:range for each lat/long/alt property,
http://www.w3.org/2001/XMLSchema#float

Revision 1.7  2003/01/10 20:25:16  danbri
Longer rdfs:comment for Point, trying to be Earth-centric and neutral about
coordinate system(s) at the same time. Feedback welcomed.

Revision 1.6  2003/01/10 20:18:30  danbri
Added CVS log comments into the RDF/XML as an rdfs:comment property of the
vocabulary. Note that this is not common practice (but seems both harmless
and potentially useful).


revision 1.5
date: 2003/01/10 20:14:31;  author: danbri;  state: Exp;  lines: +16 -5
Updated schema:
Added a dc:date, added url for more info. Changed the rdfs:label of the
namespace from gp to geo. Added a class Point, set as the rdfs:domain of
each property. Added XML comment on the lat_long property suggesting that
we might not need it (based on #rdfig commentary from implementors).

revision 1.4
date: 2003/01/10 20:01:07;  author: danbri;  state: Exp;  lines: +6 -5
Fixed typo; several rdfs:about attributes are now rdf:about. Thanks to MortenF in
#rdfig for catching this error.

revision 1.3
date: 2003/01/10 11:59:03;  author: danbri;  state: Exp;  lines: +4 -3
fixed buglet in vocab, added more wgs links

revision 1.2
date: 2003/01/10 11:01:11;  author: danbri;  state: Exp;  lines: +4 -4
Removed alt from the as-a-flat-string property, and switched from
space separated to comma separated.

revision 1.1
date: 2003/01/10 10:53:23;  author: danbri;  state: Exp;
basic geo vocab

""" ;
                                           rdfs:label "geo" .


<http://www.w3.org/2003/01/geo/wgs84_pos#lat_long> rdfs:comment "A comma-separated representation of a latitude, longitude coordinate." ;
                                                   rdfs:label "lat/long" .


<http://www.w3.org/2003/01/geo/wgs84_pos#location> rdfs:comment "The relation between something and the point,  or other geometrical thing in space, where it is.  For example, the realtionship between a radio tower and a Point with a given lat and long. Or a relationship between a park and its outline as a closed arc of points, or a road and its location as a arc (a sequence of points). Clearly in practice there will be limit to the accuracy of any such statement, but one would expect an accuracy appropriate for the size of the object and uses such as mapping ."@en ,
                                                                """The relation between something and the point, 
 or other geometrical thing in space, where it is.  For example, the realtionship between
 a radio tower and a Point with a given lat and long.
 Or a relationship between a park and its outline as a closed arc of points, or a road and
 its location as a arc (a sequence of points).
 Clearly in practice there will be limit to the accuracy of any such statement, but one would expect
 an accuracy appropriate for the size of the object and uses such as mapping .
 """ ;
                                                   rdfs:isDefinedBy <http://www.w3.org/2003/01/geo/wgs84_pos#> ;
                                                   rdfs:label "location"@en ,
                                                              "location" .


###  Generated by the OWL API (version 5.1.7) https://github.com/owlcs/owlapi/
