<?xml version="1.0"?>
<rdf:RDF xmlns="https://w3id.org/bim4eepsa#"
     xml:base="https://w3id.org/bim4eepsa"
     xmlns:owl="http://www.w3.org/2002/07/owl#"
     xmlns:xsd="http://www.w3.org/2001/XMLSchema#"
     xmlns:rdfs="http://www.w3.org/2000/01/rdf-schema#"
     xmlns:rdf="http://www.w3.org/1999/02/22-rdf-syntax-ns#"
     xmlns:terms="http://purl.org/dc/terms/"
     xmlns:xml="http://www.w3.org/XML/1998/namespace"
     xmlns:wgs84_pos="http://www.w3.org/2003/01/geo/wgs84_pos#"
     xmlns:bibo="http://purl.org/ontology/bibo/"
     xmlns:vann="http://purl.org/vocab/vann/"
     xmlns:prov="http://www.w3.org/ns/prov#"
     xmlns:foaf="http://xmlns.com/foaf/0.1/"
     xmlns:dc="http://purl.org/dc/elements/1.1/">
    <owl:Ontology rdf:about="https://w3id.org/bim4eepsa">
        <owl:versionIRI rdf:resource="https://raw.githubusercontent.com/iesnaola/eepsa/master/EEPSA_previousVersions/bim4eepsa-0.2.owl"/>
        <owl:versionInfo rdf:datatype="http://www.w3.org/2001/XMLSchema#decimal">0.2</owl:versionInfo>
        <terms:issued>2017-07-10</terms:issued>
        <dc:publisher>IK4-TEKNIKER (http://www.tekniker.es)</dc:publisher>
        <rdfs:comment xml:lang="en">Building and space-related information for the EEPSA Ontology.</rdfs:comment>
        <terms:creator xml:lang="en">Iker Esnaola-Gonzalez &lt;mailto:iker.esnaola@tekniker.es&gt;
Jesús Bermúdez &lt;mailto:jesus.bermudez@ehu.eus&gt;</terms:creator>
        <dc:title>BIM for EEPSA</dc:title>
        <terms:license xml:lang="en">This work is licensed under the Creative Commons Attribution-NonCommercial 4.0 International License. To view a copy of this license, visit http://creativecommons.org/licenses/by-nc/4.0/.</terms:license>
        <bibo:status xml:lang="en">Work in progress</bibo:status>
        <vann:preferredNamespacePrefix>bim4eepsa</vann:preferredNamespacePrefix>
    </owl:Ontology>
    


    <!-- 
    ///////////////////////////////////////////////////////////////////////////////////////
    //
    // Annotation properties
    //
    ///////////////////////////////////////////////////////////////////////////////////////
     -->

    


    <!-- http://purl.org/dc/elements/1.1/date -->

    <owl:AnnotationProperty rdf:about="http://purl.org/dc/elements/1.1/date"/>
    


    <!-- http://purl.org/dc/elements/1.1/description -->

    <owl:AnnotationProperty rdf:about="http://purl.org/dc/elements/1.1/description"/>
    


    <!-- http://purl.org/dc/elements/1.1/publisher -->

    <owl:AnnotationProperty rdf:about="http://purl.org/dc/elements/1.1/publisher"/>
    


    <!-- http://purl.org/dc/elements/1.1/title -->

    <owl:AnnotationProperty rdf:about="http://purl.org/dc/elements/1.1/title"/>
    


    <!-- http://purl.org/dc/terms/creator -->

    <owl:AnnotationProperty rdf:about="http://purl.org/dc/terms/creator"/>
    


    <!-- http://purl.org/dc/terms/issued -->

    <owl:AnnotationProperty rdf:about="http://purl.org/dc/terms/issued"/>
    


    <!-- http://purl.org/dc/terms/license -->

    <owl:AnnotationProperty rdf:about="http://purl.org/dc/terms/license"/>
    


    <!-- http://purl.org/ontology/bibo/status -->

    <owl:AnnotationProperty rdf:about="http://purl.org/ontology/bibo/status"/>
    


    <!-- http://purl.org/vocab/vann/preferredNamespacePrefix -->

    <owl:AnnotationProperty rdf:about="http://purl.org/vocab/vann/preferredNamespacePrefix"/>
    


    <!-- http://www.w3.org/2002/07/owl#versionInfo -->

    <owl:AnnotationProperty rdf:about="http://www.w3.org/2002/07/owl#versionInfo"/>
    


    <!-- http://www.w3.org/2003/01/geo/wgs84_pos#alt -->

    <owl:AnnotationProperty rdf:about="http://www.w3.org/2003/01/geo/wgs84_pos#alt">
        <rdfs:comment>The WGS84 altitude of a SpatialThing (decimal meters 
above the local reference ellipsoid).</rdfs:comment>
        <rdfs:label>altitude</rdfs:label>
        <rdfs:domain rdf:resource="http://www.w3.org/2003/01/geo/wgs84_pos#SpatialThing"/>
    </owl:AnnotationProperty>
    


    <!-- http://www.w3.org/2003/01/geo/wgs84_pos#lat -->

    <owl:AnnotationProperty rdf:about="http://www.w3.org/2003/01/geo/wgs84_pos#lat">
        <rdfs:comment>The WGS84 latitude of a SpatialThing (decimal degrees).</rdfs:comment>
        <rdfs:label>latitude</rdfs:label>
        <rdfs:domain rdf:resource="http://www.w3.org/2003/01/geo/wgs84_pos#SpatialThing"/>
    </owl:AnnotationProperty>
    


    <!-- http://www.w3.org/2003/01/geo/wgs84_pos#location -->

    <owl:AnnotationProperty rdf:about="http://www.w3.org/2003/01/geo/wgs84_pos#location">
        <rdfs:subPropertyOf rdf:resource="http://xmlns.com/foaf/0.1/based_near"/>
        <rdfs:range rdf:resource="http://www.w3.org/2003/01/geo/wgs84_pos#SpatialThing"/>
    </owl:AnnotationProperty>
    


    <!-- http://www.w3.org/2003/01/geo/wgs84_pos#long -->

    <owl:AnnotationProperty rdf:about="http://www.w3.org/2003/01/geo/wgs84_pos#long">
        <rdfs:comment>The WGS84 longitude of a SpatialThing (decimal degrees).</rdfs:comment>
        <rdfs:label>longitude</rdfs:label>
        <rdfs:domain rdf:resource="http://www.w3.org/2003/01/geo/wgs84_pos#SpatialThing"/>
    </owl:AnnotationProperty>
    


    <!-- http://www.w3.org/ns/prov#hadPrimarySource -->

    <owl:AnnotationProperty rdf:about="http://www.w3.org/ns/prov#hadPrimarySource"/>
    


    <!-- http://xmlns.com/foaf/0.1/based_near -->

    <owl:AnnotationProperty rdf:about="http://xmlns.com/foaf/0.1/based_near"/>
    


    <!-- 
    ///////////////////////////////////////////////////////////////////////////////////////
    //
    // Object Properties
    //
    ///////////////////////////////////////////////////////////////////////////////////////
     -->

    


    <!-- http://www.w3.org/2003/01/geo/wgs84_pos#location -->

    <owl:ObjectProperty rdf:about="http://www.w3.org/2003/01/geo/wgs84_pos#location"/>
    


    <!-- https://w3id.org/def/saref4bldg#contains -->

    <owl:ObjectProperty rdf:about="https://w3id.org/def/saref4bldg#contains">
        <owl:inverseOf rdf:resource="https://w3id.org/def/saref4bldg#isContainedIn"/>
        <rdf:type rdf:resource="http://www.w3.org/2002/07/owl#TransitiveProperty"/>
        <rdfs:comment xml:lang="en">A relation between a physical space and the objects located in such space.</rdfs:comment>
        <rdfs:label xml:lang="en">contains</rdfs:label>
    </owl:ObjectProperty>
    


    <!-- https://w3id.org/def/saref4bldg#hasSpace -->

    <owl:ObjectProperty rdf:about="https://w3id.org/def/saref4bldg#hasSpace">
        <owl:inverseOf rdf:resource="https://w3id.org/def/saref4bldg#isSpaceOf"/>
        <rdf:type rdf:resource="http://www.w3.org/2002/07/owl#TransitiveProperty"/>
        <rdfs:comment xml:lang="en">Relation between a building or a building space and the spaces it can be divided into.</rdfs:comment>
        <rdfs:label xml:lang="en">has space</rdfs:label>
    </owl:ObjectProperty>
    


    <!-- https://w3id.org/def/saref4bldg#isContainedIn -->

    <owl:ObjectProperty rdf:about="https://w3id.org/def/saref4bldg#isContainedIn">
        <rdf:type rdf:resource="http://www.w3.org/2002/07/owl#TransitiveProperty"/>
        <rdfs:comment xml:lang="en">A relation between an object and the physical space in which it is located.</rdfs:comment>
        <rdfs:label xml:lang="en">is contained in</rdfs:label>
    </owl:ObjectProperty>
    


    <!-- https://w3id.org/def/saref4bldg#isSpaceOf -->

    <owl:ObjectProperty rdf:about="https://w3id.org/def/saref4bldg#isSpaceOf">
        <rdf:type rdf:resource="http://www.w3.org/2002/07/owl#TransitiveProperty"/>
        <rdfs:comment xml:lang="en">Relation between a building space and the building or building space it belongs to.</rdfs:comment>
        <rdfs:label xml:lang="en">isSpaceOf</rdfs:label>
    </owl:ObjectProperty>
    


    <!-- 
    ///////////////////////////////////////////////////////////////////////////////////////
    //
    // Data properties
    //
    ///////////////////////////////////////////////////////////////////////////////////////
     -->

    


    <!-- https://w3id.org/bim4eepsa#pset_BuildingCommon_buildingID -->

    <owl:DatatypeProperty rdf:about="https://w3id.org/bim4eepsa#pset_BuildingCommon_buildingID">
        <rdfs:range rdf:resource="http://www.w3.org/2001/XMLSchema#string"/>
        <rdfs:comment xml:lang="en">A unique identifier assigned to a building. A temporary identifier is initially assigned at the time of making a planning application. This temporary identifier is changed to a permanent identifier when the building is registered into a statutory buildings and properties database.</rdfs:comment>
        <rdfs:label xml:lang="en">Building ID</rdfs:label>
    </owl:DatatypeProperty>
    


    <!-- https://w3id.org/bim4eepsa#pset_BuildingCommon_constructionMethod -->

    <owl:DatatypeProperty rdf:about="https://w3id.org/bim4eepsa#pset_BuildingCommon_constructionMethod">
        <rdfs:range rdf:resource="http://www.w3.org/2001/XMLSchema#string"/>
        <rdfs:comment xml:lang="en">The type of intervention on the building: new construction, renovation, rehabilitation, etc.</rdfs:comment>
        <rdfs:label xml:lang="en">Construction method</rdfs:label>
    </owl:DatatypeProperty>
    


    <!-- https://w3id.org/bim4eepsa#pset_BuildingCommon_fireProtectionClass -->

    <owl:DatatypeProperty rdf:about="https://w3id.org/bim4eepsa#pset_BuildingCommon_fireProtectionClass">
        <rdfs:range rdf:resource="http://www.w3.org/2001/XMLSchema#string"/>
        <rdfs:comment xml:lang="en">Main fire protection class for the building which is assigned from the fire protection classification table as given by the relevant national building code.</rdfs:comment>
        <rdfs:label xml:lang="en">Fire protection class</rdfs:label>
    </owl:DatatypeProperty>
    


    <!-- https://w3id.org/bim4eepsa#pset_BuildingCommon_grossPlannedArea -->

    <owl:DatatypeProperty rdf:about="https://w3id.org/bim4eepsa#pset_BuildingCommon_grossPlannedArea">
        <rdfs:range rdf:resource="http://www.w3.org/2001/XMLSchema#double"/>
        <rdfs:comment xml:lang="en">Total planned gross area for the building Used for programming the building.</rdfs:comment>
        <rdfs:label xml:lang="en">Gross planned area</rdfs:label>
    </owl:DatatypeProperty>
    


    <!-- https://w3id.org/bim4eepsa#pset_BuildingCommon_netPlannedArea -->

    <owl:DatatypeProperty rdf:about="https://w3id.org/bim4eepsa#pset_BuildingCommon_netPlannedArea">
        <rdfs:range rdf:resource="http://www.w3.org/2001/XMLSchema#double"/>
        <rdfs:comment xml:lang="en">Total planned net area for the building Used for programming the building.</rdfs:comment>
        <rdfs:label xml:lang="en">Net planned area</rdfs:label>
    </owl:DatatypeProperty>
    


    <!-- https://w3id.org/bim4eepsa#pset_BuildingCommon_numberOfStoreys -->

    <owl:DatatypeProperty rdf:about="https://w3id.org/bim4eepsa#pset_BuildingCommon_numberOfStoreys">
        <rdfs:range rdf:resource="http://www.w3.org/2001/XMLSchema#integer"/>
        <rdfs:comment xml:lang="en">The number of storeys within a building. Captured for those cases where the IfcBuildingStorey entity is not used. Note that if IfcBuilingStorey is asserted and the number of storeys in a building can be determined from it, then this approach should be used in preference to setting a property for the number of storeys.</rdfs:comment>
        <rdfs:label xml:lang="en">Number of storeys</rdfs:label>
    </owl:DatatypeProperty>
    


    <!-- https://w3id.org/bim4eepsa#pset_BuildingCommon_occupancyType -->

    <owl:DatatypeProperty rdf:about="https://w3id.org/bim4eepsa#pset_BuildingCommon_occupancyType">
        <rdfs:range rdf:resource="http://www.w3.org/2001/XMLSchema#string"/>
        <rdfs:comment xml:lang="en">Occupancy type for this object. It is defined according to the presiding national building code.</rdfs:comment>
        <rdfs:label xml:lang="en">Occupancy type</rdfs:label>
    </owl:DatatypeProperty>
    


    <!-- https://w3id.org/bim4eepsa#pset_BuildingCommon_yearOfConstruction -->

    <owl:DatatypeProperty rdf:about="https://w3id.org/bim4eepsa#pset_BuildingCommon_yearOfConstruction">
        <rdfs:range rdf:resource="http://www.w3.org/2001/XMLSchema#integer"/>
        <rdfs:comment xml:lang="en">Year of construction of this building, including expected year of completion.</rdfs:comment>
        <rdfs:label xml:lang="en">Year of construction</rdfs:label>
    </owl:DatatypeProperty>
    


    <!-- https://w3id.org/bim4eepsa#pset_BuildingCommon_yearOfLastRefurbishment -->

    <owl:DatatypeProperty rdf:about="https://w3id.org/bim4eepsa#pset_BuildingCommon_yearOfLastRefurbishment">
        <rdfs:range rdf:resource="http://www.w3.org/2001/XMLSchema#integer"/>
        <rdfs:comment xml:lang="en">Year of last major refurbishment, or reconstruction, of the building (applies to reconstruction works).</rdfs:comment>
        <rdfs:label xml:lang="en">Year of last refurbishment</rdfs:label>
    </owl:DatatypeProperty>
    


    <!-- https://w3id.org/bim4eepsa#pset_BuildingUse_marketCategory -->

    <owl:DatatypeProperty rdf:about="https://w3id.org/bim4eepsa#pset_BuildingUse_marketCategory">
        <rdfs:comment xml:lang="en">Category of use e.g. residential, commercial, recreation etc.</rdfs:comment>
        <rdfs:label xml:lang="en">Market category</rdfs:label>
    </owl:DatatypeProperty>
    


    <!-- https://w3id.org/bim4eepsa#pset_BuildingUse_marketSubCategory -->

    <owl:DatatypeProperty rdf:about="https://w3id.org/bim4eepsa#pset_BuildingUse_marketSubCategory">
        <rdfs:comment xml:lang="en">Subset of category of use e.g. multi-family, 2 bedroom, low rise.</rdfs:comment>
        <rdfs:label xml:lang="en">Market sub category</rdfs:label>
    </owl:DatatypeProperty>
    


    <!-- https://w3id.org/bim4eepsa#pset_BuildingUse_narrativeText -->

    <owl:DatatypeProperty rdf:about="https://w3id.org/bim4eepsa#pset_BuildingUse_narrativeText">
        <rdfs:comment xml:lang="en">Added information relating to the adjacent building use that is not appropriate to the general descriptive text associated with an entity through the inherited IfcRoot.Description.</rdfs:comment>
        <rdfs:label xml:lang="en">Narrative text</rdfs:label>
    </owl:DatatypeProperty>
    


    <!-- https://w3id.org/bim4eepsa#pset_BuildingUse_planningControlStatus -->

    <owl:DatatypeProperty rdf:about="https://w3id.org/bim4eepsa#pset_BuildingUse_planningControlStatus">
        <rdfs:comment xml:lang="en">Label of zoning category or class, or planning control category for the site or facility.</rdfs:comment>
        <rdfs:label xml:lang="en">Planning control status</rdfs:label>
    </owl:DatatypeProperty>
    


    <!-- 
    ///////////////////////////////////////////////////////////////////////////////////////
    //
    // Classes
    //
    ///////////////////////////////////////////////////////////////////////////////////////
     -->

    


    <!-- http://www.w3.org/2003/01/geo/wgs84_pos#Point -->

    <owl:Class rdf:about="http://www.w3.org/2003/01/geo/wgs84_pos#Point">
        <rdfs:subClassOf rdf:resource="http://www.w3.org/2003/01/geo/wgs84_pos#SpatialThing"/>
        <rdfs:comment> 
Uniquely identified by lat/long/alt. i.e.

spaciallyIntersects(P1, P2) :- lat(P1, LAT), long(P1, LONG), alt(P1, ALT),
  lat(P2, LAT), long(P2, LONG), alt(P2, ALT).

sameThing(P1, P2) :- type(P1, Point), type(P2, Point), spaciallyIntersects(P1, P2).
  </rdfs:comment>
        <rdfs:comment>A point, typically described using a coordinate system relative to Earth, such as WGS84.
  </rdfs:comment>
        <rdfs:label>point</rdfs:label>
    </owl:Class>
    


    <!-- http://www.w3.org/2003/01/geo/wgs84_pos#SpatialThing -->

    <owl:Class rdf:about="http://www.w3.org/2003/01/geo/wgs84_pos#SpatialThing">
        <rdfs:comment>Anything with spatial extent, i.e. size, shape, or position.
 e.g. people, places, bowling balls, as well as abstract areas like cubes.
</rdfs:comment>
        <rdfs:comment xml:lang="en">Anything with spatial extent, i.e. size, shape, or position. e.g. people, places, bowling balls, as well as abstract areas like cubes.</rdfs:comment>
        <rdfs:isDefinedBy rdf:resource="http://www.w3.org/2003/01/geo/wgs84_pos#"/>
        <rdfs:label xml:lang="en">Spatial thing</rdfs:label>
        <rdfs:label>SpatialThing</rdfs:label>
    </owl:Class>
    


    <!-- https://w3id.org/bim4eepsa#BuildingElement -->

    <owl:Class rdf:about="https://w3id.org/bim4eepsa#BuildingElement">
        <rdfs:subClassOf rdf:resource="https://w3id.org/def/saref4bldg#PhysicalObject"/>
        <rdfs:comment xml:lang="en">The building element comprises all elements that are primarily part of the construction of a building, i.e., its structural and space separating system.</rdfs:comment>
        <rdfs:label xml:lang="en">Building Element</rdfs:label>
        <rdfs:seeAlso rdf:resource="http://ifcowl.openbimstandards.org/IFC4_ADD2#IfcBuildingElement"/>
    </owl:Class>
    


    <!-- https://w3id.org/bim4eepsa#Door -->

    <owl:Class rdf:about="https://w3id.org/bim4eepsa#Door">
        <rdfs:subClassOf rdf:resource="https://w3id.org/bim4eepsa#BuildingElement"/>
        <rdfs:comment xml:lang="en">Definition according to ISO 6707-1: construction for closing an opening, intended primarily for access with hinged, pivoted or sliding operation.</rdfs:comment>
        <rdfs:label xml:lang="en">Door</rdfs:label>
        <rdfs:seeAlso rdf:resource="http://ifcowl.openbimstandards.org/IFC4_ADD2#IfcDoor"/>
    </owl:Class>
    


    <!-- https://w3id.org/bim4eepsa#ExternalBuildingElement -->

    <owl:Class rdf:about="https://w3id.org/bim4eepsa#ExternalBuildingElement">
        <rdfs:subClassOf rdf:resource="https://w3id.org/bim4eepsa#BuildingElement"/>
        <rdfs:comment xml:lang="en">A building element that is external (face the outside of the building)</rdfs:comment>
        <rdfs:label xml:lang="en">External building element</rdfs:label>
    </owl:Class>
    


    <!-- https://w3id.org/bim4eepsa#ExternalDoor -->

    <owl:Class rdf:about="https://w3id.org/bim4eepsa#ExternalDoor">
        <owl:equivalentClass>
            <owl:Class>
                <owl:intersectionOf rdf:parseType="Collection">
                    <rdf:Description rdf:about="https://w3id.org/bim4eepsa#Door"/>
                    <rdf:Description rdf:about="https://w3id.org/bim4eepsa#ExternalBuildingElement"/>
                </owl:intersectionOf>
            </owl:Class>
        </owl:equivalentClass>
        <rdfs:subClassOf rdf:resource="https://w3id.org/bim4eepsa#Door"/>
        <rdfs:label xml:lang="en">External door</rdfs:label>
        <rdfs:seeAlso xml:lang="en">A door that is external (facing the outside of the building)</rdfs:seeAlso>
    </owl:Class>
    


    <!-- https://w3id.org/bim4eepsa#ExternalWall -->

    <owl:Class rdf:about="https://w3id.org/bim4eepsa#ExternalWall">
        <owl:equivalentClass>
            <owl:Class>
                <owl:intersectionOf rdf:parseType="Collection">
                    <rdf:Description rdf:about="https://w3id.org/bim4eepsa#ExternalBuildingElement"/>
                    <rdf:Description rdf:about="https://w3id.org/bim4eepsa#Wall"/>
                </owl:intersectionOf>
            </owl:Class>
        </owl:equivalentClass>
        <rdfs:subClassOf rdf:resource="https://w3id.org/bim4eepsa#Wall"/>
        <rdfs:label xml:lang="en">External wall</rdfs:label>
        <rdfs:seeAlso xml:lang="en">A wall that is external (facing the outside of the building)</rdfs:seeAlso>
    </owl:Class>
    


    <!-- https://w3id.org/bim4eepsa#ExternalWindow -->

    <owl:Class rdf:about="https://w3id.org/bim4eepsa#ExternalWindow">
        <owl:equivalentClass>
            <owl:Class>
                <owl:intersectionOf rdf:parseType="Collection">
                    <rdf:Description rdf:about="https://w3id.org/bim4eepsa#ExternalBuildingElement"/>
                    <rdf:Description rdf:about="https://w3id.org/bim4eepsa#Window"/>
                </owl:intersectionOf>
            </owl:Class>
        </owl:equivalentClass>
        <rdfs:subClassOf rdf:resource="https://w3id.org/bim4eepsa#Window"/>
        <rdfs:comment xml:lang="en">A window that is external (facing the outside of the building)</rdfs:comment>
        <rdfs:label xml:lang="en">External window</rdfs:label>
    </owl:Class>
    


    <!-- https://w3id.org/bim4eepsa#Roof -->

    <owl:Class rdf:about="https://w3id.org/bim4eepsa#Roof">
        <rdfs:subClassOf rdf:resource="https://w3id.org/bim4eepsa#BuildingElement"/>
        <rdfs:comment xml:lang="en">Definition according to ISO 6707-1: construction enclosing the building from above.</rdfs:comment>
        <rdfs:label xml:lang="en">Roof</rdfs:label>
        <rdfs:seeAlso rdf:resource="http://ifcowl.openbimstandards.org/IFC4_ADD2#IfcRoof"/>
    </owl:Class>
    


    <!-- https://w3id.org/bim4eepsa#Skylight -->

    <owl:Class rdf:about="https://w3id.org/bim4eepsa#Skylight">
        <rdfs:subClassOf rdf:resource="https://w3id.org/bim4eepsa#BuildingElement"/>
        <rdfs:label xml:lang="en">Skylight</rdfs:label>
        <rdfs:seeAlso xml:lang="en">Skylights are light transmitting fenestration (elements filling building envelope openings) forming all, or a portion of, the roof of a building&apos;s space for daylighting purposes. (Wikipedia)</rdfs:seeAlso>
    </owl:Class>
    


    <!-- https://w3id.org/bim4eepsa#Wall -->

    <owl:Class rdf:about="https://w3id.org/bim4eepsa#Wall">
        <rdfs:subClassOf rdf:resource="https://w3id.org/bim4eepsa#BuildingElement"/>
        <rdfs:comment xml:lang="en">Definition according to ISO 6707-1: vertical construction usually in masonry or in concrete which bounds or subdivides a construction works and fulfils a load bearing or retaining function.</rdfs:comment>
        <rdfs:label xml:lang="en">Wall</rdfs:label>
        <rdfs:seeAlso rdf:resource="http://ifcowl.openbimstandards.org/IFC4_ADD2#IfcWall"/>
    </owl:Class>
    


    <!-- https://w3id.org/bim4eepsa#WeatherStation -->

    <owl:Class rdf:about="https://w3id.org/bim4eepsa#WeatherStation">
        <rdfs:subClassOf rdf:resource="https://w3id.org/def/saref4bldg#Building"/>
        <rdfs:comment xml:lang="en">A weather station is a facility, either on land or sea, with instruments and equipment for measuring atmospheric conditions to provide information for weather forecasts and to study the weather and climate (Wikipedia)</rdfs:comment>
        <rdfs:label rdf:resource="http://aemet.linkeddata.es/ontology/WeatherStation"/>
        <rdfs:label xml:lang="en">Weather station</rdfs:label>
    </owl:Class>
    


    <!-- https://w3id.org/bim4eepsa#Window -->

    <owl:Class rdf:about="https://w3id.org/bim4eepsa#Window">
        <rdfs:subClassOf rdf:resource="https://w3id.org/bim4eepsa#BuildingElement"/>
        <rdfs:comment xml:lang="en">Definition according to ISO 6707-1: Construction for closing a vertical or near vertical opening in a wall or pitched roof that will admit light and may admit fresh air.</rdfs:comment>
        <rdfs:label xml:lang="en">Window</rdfs:label>
        <rdfs:seeAlso rdf:resource="http://ifcowl.openbimstandards.org/IFC4_ADD2#IfcWindow"/>
    </owl:Class>
    


    <!-- https://w3id.org/def/saref4bldg#Building -->

    <owl:Class rdf:about="https://w3id.org/def/saref4bldg#Building">
        <rdfs:subClassOf rdf:resource="http://www.w3.org/2003/01/geo/wgs84_pos#SpatialThing"/>
        <rdfs:subClassOf>
            <owl:Restriction>
                <owl:onProperty rdf:resource="http://www.w3.org/2003/01/geo/wgs84_pos#location"/>
                <owl:allValuesFrom rdf:resource="http://www.w3.org/2003/01/geo/wgs84_pos#SpatialThing"/>
            </owl:Restriction>
        </rdfs:subClassOf>
        <rdfs:subClassOf>
            <owl:Restriction>
                <owl:onProperty rdf:resource="https://w3id.org/def/saref4bldg#hasSpace"/>
                <owl:allValuesFrom rdf:resource="https://w3id.org/def/saref4bldg#BuildingSpace"/>
            </owl:Restriction>
        </rdfs:subClassOf>
        <rdfs:subClassOf>
            <owl:Restriction>
                <owl:onProperty rdf:resource="https://w3id.org/bim4eepsa#pset_BuildingCommon_buildingID"/>
                <owl:allValuesFrom rdf:resource="http://www.w3.org/2001/XMLSchema#string"/>
            </owl:Restriction>
        </rdfs:subClassOf>
        <rdfs:subClassOf>
            <owl:Restriction>
                <owl:onProperty rdf:resource="https://w3id.org/bim4eepsa#pset_BuildingCommon_numberOfStoreys"/>
                <owl:allValuesFrom rdf:resource="http://www.w3.org/2001/XMLSchema#integer"/>
            </owl:Restriction>
        </rdfs:subClassOf>
        <rdfs:subClassOf>
            <owl:Restriction>
                <owl:onProperty rdf:resource="https://w3id.org/bim4eepsa#pset_BuildingCommon_occupancyType"/>
                <owl:allValuesFrom rdf:resource="http://www.w3.org/2001/XMLSchema#string"/>
            </owl:Restriction>
        </rdfs:subClassOf>
        <rdfs:comment xml:lang="en">A building represents a structure that provides shelter for its occupants or contents and stands in one place. The building is also used to provide a basic element within the spatial structure hierarchy for the components of a building project (together with site, storey, and space).</rdfs:comment>
        <rdfs:label xml:lang="en">Building</rdfs:label>
        <rdfs:seeAlso rdf:resource="https://w3id.org/ifc/IFC4_ADD1#IfcBuilding"/>
        <prov:hadPrimarySource rdf:resource="http://www.buildingsmart-tech.org/ifc/IFC4/Add1/html/schema/ifcproductextension/lexical/ifcbuilding.htm"/>
    </owl:Class>
    


    <!-- https://w3id.org/def/saref4bldg#BuildingSpace -->

    <owl:Class rdf:about="https://w3id.org/def/saref4bldg#BuildingSpace">
        <rdfs:subClassOf rdf:resource="http://www.w3.org/2003/01/geo/wgs84_pos#SpatialThing"/>
        <rdfs:subClassOf>
            <owl:Restriction>
                <owl:onProperty rdf:resource="https://w3id.org/def/saref4bldg#contains"/>
                <owl:allValuesFrom rdf:resource="https://w3id.org/def/saref4bldg#PhysicalObject"/>
            </owl:Restriction>
        </rdfs:subClassOf>
        <rdfs:subClassOf>
            <owl:Restriction>
                <owl:onProperty rdf:resource="https://w3id.org/def/saref4bldg#hasSpace"/>
                <owl:allValuesFrom rdf:resource="https://w3id.org/def/saref4bldg#BuildingSpace"/>
            </owl:Restriction>
        </rdfs:subClassOf>
        <rdfs:subClassOf>
            <owl:Restriction>
                <owl:onProperty rdf:resource="https://w3id.org/def/saref4bldg#isSpaceOf"/>
                <owl:allValuesFrom>
                    <owl:Class>
                        <owl:unionOf rdf:parseType="Collection">
                            <rdf:Description rdf:about="https://w3id.org/def/saref4bldg#Building"/>
                            <rdf:Description rdf:about="https://w3id.org/def/saref4bldg#BuildingSpace"/>
                        </owl:unionOf>
                    </owl:Class>
                </owl:allValuesFrom>
            </owl:Restriction>
        </rdfs:subClassOf>
        <rdfs:comment xml:lang="en">An entity used to define the physical spaces of the building. A building space contains devices or building objects.</rdfs:comment>
        <rdfs:label xml:lang="en">Building space</rdfs:label>
    </owl:Class>
    


    <!-- https://w3id.org/def/saref4bldg#PhysicalObject -->

    <owl:Class rdf:about="https://w3id.org/def/saref4bldg#PhysicalObject">
        <rdfs:subClassOf rdf:resource="http://www.w3.org/2003/01/geo/wgs84_pos#SpatialThing"/>
        <rdfs:subClassOf>
            <owl:Restriction>
                <owl:onProperty rdf:resource="http://www.w3.org/2003/01/geo/wgs84_pos#location"/>
                <owl:allValuesFrom rdf:resource="http://www.w3.org/2003/01/geo/wgs84_pos#SpatialThing"/>
            </owl:Restriction>
        </rdfs:subClassOf>
        <rdfs:subClassOf>
            <owl:Restriction>
                <owl:onProperty rdf:resource="https://w3id.org/def/saref4bldg#contains"/>
                <owl:allValuesFrom rdf:resource="https://w3id.org/def/saref4bldg#PhysicalObject"/>
            </owl:Restriction>
        </rdfs:subClassOf>
        <rdfs:subClassOf>
            <owl:Restriction>
                <owl:onProperty rdf:resource="https://w3id.org/def/saref4bldg#isContainedIn"/>
                <owl:allValuesFrom>
                    <owl:Class>
                        <owl:unionOf rdf:parseType="Collection">
                            <rdf:Description rdf:about="https://w3id.org/def/saref4bldg#BuildingSpace"/>
                            <rdf:Description rdf:about="https://w3id.org/def/saref4bldg#PhysicalObject"/>
                        </owl:unionOf>
                    </owl:Class>
                </owl:allValuesFrom>
            </owl:Restriction>
        </rdfs:subClassOf>
        <rdfs:comment xml:lang="en">Any Object that has a proper space region.  (Definition extracted from DUL ontology)</rdfs:comment>
        <rdfs:label xml:lang="en">Physical object</rdfs:label>
    </owl:Class>
    


    <!-- 
    ///////////////////////////////////////////////////////////////////////////////////////
    //
    // Annotations
    //
    ///////////////////////////////////////////////////////////////////////////////////////
     -->

    <rdf:Description rdf:about="http://www.w3.org/2003/01/geo/wgs84_pos#">
        <dc:date>$Date: 2009/04/20 15:00:30 $</dc:date>
        <rdfs:label>geo</rdfs:label>
        <dc:description>A vocabulary for representing latitude, longitude and 
 altitude information in the WGS84 geodetic reference datum. 
 Version $Id: wgs84_pos.rdf,v 1.22 2009/04/20 15:00:30 timbl Exp $. See http://www.w3.org/2003/01/geo/ for more details.</dc:description>
        <rdfs:comment>
Recent changes to this namespace:
$Log: wgs84_pos.rdf,v $
Revision 1.22  2009/04/20 15:00:30  timbl
Remove the time bits which have been deal with elsewhere eg in iCal.

Revision 1.21  2009/04/20 12:52:47  timbl
try again

Revision 1.20  2009/04/20 12:42:11  timbl
Add Event (edited ages ago and never checked in), and location (following discussion http://chatlogs.planetrdf.com/swig/2009-04-20#T12-36-09)

Revision 1.19  2009/04/20 12:36:31  timbl
Add Event (edited ages ago and never checked in), and location (following discussion http://chatlogs.planetrdf.com/swig/2009-04-20#T12-36-09)

Revision 1.18  2006/02/01 22:01:04  danbri
Clarified that lat and long are decimal degrees, and that alt is decimal metres about local reference ellipsoid

Revision 1.17  2004/02/06 17:38:12  danbri
Fixed a bad commit screwup

Revision 1.15  2003/04/19 11:24:08  danbri
Fixed the typo even more.

Revision 1.14  2003/04/19 11:16:56  danbri
fixed a typo

Revision 1.13  2003/02/19 22:27:27  connolly
relaxed domain constraints on lat/long/alt from Point to SpatialThing

Revision 1.12  2003/01/12 01:41:41  danbri
Trying local copy of XSLT doc.

Revision 1.11  2003/01/12 01:20:18  danbri
added a link to morten&apos;s xslt rdfs viewer.

Revision 1.10  2003/01/11 18:56:49  danbri
Removed datatype range from lat and long properties, since they would
have required each occurance of the property to mention the datatype.

Revision 1.9  2003/01/11 11:41:31  danbri
Another typo; repaired rdfs:Property to rdf:Property x4

Revision 1.8  2003/01/11 11:05:02  danbri
Added an rdfs:range for each lat/long/alt property,
http://www.w3.org/2001/XMLSchema#float

Revision 1.7  2003/01/10 20:25:16  danbri
Longer rdfs:comment for Point, trying to be Earth-centric and neutral about
coordinate system(s) at the same time. Feedback welcomed.

Revision 1.6  2003/01/10 20:18:30  danbri
Added CVS log comments into the RDF/XML as an rdfs:comment property of the
vocabulary. Note that this is not common practice (but seems both harmless
and potentially useful).


revision 1.5
date: 2003/01/10 20:14:31;  author: danbri;  state: Exp;  lines: +16 -5
Updated schema:
Added a dc:date, added url for more info. Changed the rdfs:label of the
namespace from gp to geo. Added a class Point, set as the rdfs:domain of
each property. Added XML comment on the lat_long property suggesting that
we might not need it (based on #rdfig commentary from implementors).

revision 1.4
date: 2003/01/10 20:01:07;  author: danbri;  state: Exp;  lines: +6 -5
Fixed typo; several rdfs:about attributes are now rdf:about. Thanks to MortenF in
#rdfig for catching this error.

revision 1.3
date: 2003/01/10 11:59:03;  author: danbri;  state: Exp;  lines: +4 -3
fixed buglet in vocab, added more wgs links

revision 1.2
date: 2003/01/10 11:01:11;  author: danbri;  state: Exp;  lines: +4 -4
Removed alt from the as-a-flat-string property, and switched from
space separated to comma separated.

revision 1.1
date: 2003/01/10 10:53:23;  author: danbri;  state: Exp;
basic geo vocab

</rdfs:comment>
        <dc:title>WGS84 Geo Positioning: an RDF vocabulary</dc:title>
    </rdf:Description>
    <rdf:Description rdf:about="http://www.w3.org/2003/01/geo/wgs84_pos#lat_long">
        <rdfs:comment>A comma-separated representation of a latitude, longitude coordinate.</rdfs:comment>
        <rdfs:label>lat/long</rdfs:label>
    </rdf:Description>
    <rdf:Description rdf:about="http://www.w3.org/2003/01/geo/wgs84_pos#location">
        <rdfs:isDefinedBy rdf:resource="http://www.w3.org/2003/01/geo/wgs84_pos#"/>
        <rdfs:label>location</rdfs:label>
        <rdfs:comment>The relation between something and the point, 
 or other geometrical thing in space, where it is.  For example, the realtionship between
 a radio tower and a Point with a given lat and long.
 Or a relationship between a park and its outline as a closed arc of points, or a road and
 its location as a arc (a sequence of points).
 Clearly in practice there will be limit to the accuracy of any such statement, but one would expect
 an accuracy appropriate for the size of the object and uses such as mapping .
 </rdfs:comment>
        <rdfs:comment xml:lang="en">The relation between something and the point,  or other geometrical thing in space, where it is.  For example, the realtionship between a radio tower and a Point with a given lat and long. Or a relationship between a park and its outline as a closed arc of points, or a road and its location as a arc (a sequence of points). Clearly in practice there will be limit to the accuracy of any such statement, but one would expect an accuracy appropriate for the size of the object and uses such as mapping .</rdfs:comment>
        <rdfs:label xml:lang="en">location</rdfs:label>
    </rdf:Description>
</rdf:RDF>



<!-- Generated by the OWL API (version 4.2.6.20160910-2108) https://github.com/owlcs/owlapi -->

