@prefix : <https://w3id.org/datamining4eepsa#> .
@prefix owl: <http://www.w3.org/2002/07/owl#> .
@prefix rdf: <http://www.w3.org/1999/02/22-rdf-syntax-ns#> .
@prefix xml: <http://www.w3.org/XML/1998/namespace> .
@prefix xsd: <http://www.w3.org/2001/XMLSchema#> .
@prefix rdfs: <http://www.w3.org/2000/01/rdf-schema#> .
@base <https://w3id.org/datamining4eepsa> .

<https://w3id.org/datamining4eepsa> rdf:type owl:Ontology ;
                                     owl:versionIRI <https://raw.githubusercontent.com/iesnaola/eepsa/master/EEPSA_previousVersions/datamining4eepsa-0.1.owl> ;
                                     <http://creativecommons.org/ns#license> <http://creativecommons.org/licenses/by-nc/4.0/> ;
                                     <http://purl.org/dc/elements/1.1/publisher> "IK4-TEKNIKER (http://www.tekniker.es)" ;
                                     <http://purl.org/dc/terms/creator> """Iker Esnaola-Gonzalez <mailto:iker.esnaola@tekniker.es>
Jesús Bermúdez <mailto:jesus.bermudez@ehu.eus>"""@en ;
                                     <http://purl.org/dc/terms/description> "Data Mining-related knowledge representation for the EEPSA Ontology."@en ;
                                     <http://purl.org/dc/terms/issued> "2018-04-19" ;
                                     <http://purl.org/dc/terms/modified> "2018-04-19"@en ;
                                     <http://purl.org/dc/terms/title> "Data Mining for EEPSA" ;
                                     <http://purl.org/ontology/bibo/status> "Work in progress"@en ;
                                     <http://purl.org/vocab/vann/preferredNamespacePrefix> "dm4eepsa"@en ;
                                     owl:versionInfo "0.1"@en .

#################################################################
#    Annotation properties
#################################################################

###  http://creativecommons.org/ns#license
<http://creativecommons.org/ns#license> rdf:type owl:AnnotationProperty .


###  http://purl.org/dc/elements/1.1/date
<http://purl.org/dc/elements/1.1/date> rdf:type owl:AnnotationProperty .


###  http://purl.org/dc/elements/1.1/publisher
<http://purl.org/dc/elements/1.1/publisher> rdf:type owl:AnnotationProperty .


###  http://purl.org/dc/terms/creator
<http://purl.org/dc/terms/creator> rdf:type owl:AnnotationProperty .


###  http://purl.org/dc/terms/issued
<http://purl.org/dc/terms/issued> rdf:type owl:AnnotationProperty .


###  http://purl.org/dc/terms/license
<http://purl.org/dc/terms/license> rdf:type owl:AnnotationProperty .


###  http://purl.org/ontology/bibo/status
<http://purl.org/ontology/bibo/status> rdf:type owl:AnnotationProperty .


###  http://purl.org/vocab/vann/preferredNamespacePrefix
<http://purl.org/vocab/vann/preferredNamespacePrefix> rdf:type owl:AnnotationProperty .


###  http://www.w3.org/2002/07/owl#versionInfo
owl:versionInfo rdf:type owl:AnnotationProperty .


###  http://www.w3.org/ns/prov#hadPrimarySource
<http://www.w3.org/ns/prov#hadPrimarySource> rdf:type owl:AnnotationProperty .


#################################################################
#    Datatypes
#################################################################

###  http://www.w3.org/2001/XMLSchema#time
xsd:time rdf:type rdfs:Datatype .


#################################################################
#    Object Properties
#################################################################

###  https://w3id.org/datamining4eepsa#hasSolvingProcedure
:hasSolvingProcedure rdf:type owl:ObjectProperty ;
                     rdfs:range <http://www.w3.org/ns/sosa/Procedure> ;
                     <http://purl.org/ontology/bibo/status> "stable"@en ;
                     rdfs:comment "A relation between a Thing and a Procedure proposed to solve it."@en ;
                     rdfs:isDefinedBy : ;
                     rdfs:label "has solving procedure"@en .


###  https://w3id.org/datamining4eepsa#requiresImputationProcedure
:requiresImputationProcedure rdf:type owl:ObjectProperty ;
                             rdfs:subPropertyOf :hasSolvingProcedure ;
                             rdfs:range :ImputationProcedure ;
                             <http://purl.org/ontology/bibo/status> "testing"@en ;
                             rdfs:comment "The relationship between a Missing Value (chunk) and a suggested Imputation procedure to impute its value accurately."@en ;
                             rdfs:isDefinedBy : ;
                             rdfs:label "requires imputation procedure"@en .


###  https://w3id.org/datamining4eepsa#susceptibleToOutlier
:susceptibleToOutlier rdf:type owl:ObjectProperty ;
                      <http://purl.org/ontology/bibo/status> "testing"@en ;
                      rdfs:comment "The relationship between a thing (normally a device) and an Outlier it may be susceptible to."@en ;
                      rdfs:isDefinedBy : ;
                      rdfs:label "susceptible to outlier"@en .


#################################################################
#    Classes
#################################################################

###  http://www.w3.org/ns/sosa/Observation
<http://www.w3.org/ns/sosa/Observation> rdf:type owl:Class .


###  http://www.w3.org/ns/sosa/Procedure
<http://www.w3.org/ns/sosa/Procedure> rdf:type owl:Class .


###  https://w3id.org/datamining4eepsa#ComplexValueDrawing
:ComplexValueDrawing rdf:type owl:Class ;
                     rdfs:subClassOf :ValueDrawingProcedure ;
                     <http://purl.org/ontology/bibo/status> "testing"@en ;
                     rdfs:comment "Complex Value Drawing procedure to impute a Missing Value."@en ;
                     rdfs:isDefinedBy : ;
                     rdfs:label "Complex Value Drawing"@en .


###  https://w3id.org/datamining4eepsa#DeviceRelocation
:DeviceRelocation rdf:type owl:Class ;
                  rdfs:subClassOf :ProcedureUponDevice ;
                  <http://purl.org/ontology/bibo/status> "testing"@en ;
                  rdfs:comment "A procedure that consists in placing the sensing device in an adequate location."@en ;
                  rdfs:isDefinedBy : ;
                  rdfs:label "Device Relocation"@en .


###  https://w3id.org/datamining4eepsa#DeviceReplacement
:DeviceReplacement rdf:type owl:Class ;
                   rdfs:subClassOf :ProcedureUponDevice ;
                   <http://purl.org/ontology/bibo/status> "stable"@en ;
                   rdfs:comment "A procedure that consists in replacing the sensing device for another one."@en ;
                   rdfs:isDefinedBy : ;
                   rdfs:label "Device Replacement"@en .


###  https://w3id.org/datamining4eepsa#DeviceShelter
:DeviceShelter rdf:type owl:Class ;
               rdfs:subClassOf :ProcedureUponDevice ;
               <http://purl.org/ontology/bibo/status> "stable"@en ;
               rdfs:comment "A procedure that consists in covering the sensing device adequately to avoid erroneous observations. For example, Stevenson Screen to shield the sensing device against direct precipitation or direct sunlight."@en ;
               rdfs:isDefinedBy : ;
               rdfs:label "Device Shelter"@en .


###  https://w3id.org/datamining4eepsa#ImputationProcedure
:ImputationProcedure rdf:type owl:Class ;
                     rdfs:subClassOf <http://www.w3.org/ns/sosa/Procedure> ;
                     <http://purl.org/ontology/bibo/status> "stable"@en ;
                     rdfs:comment "Procedure that attempts to compute an accurate estimation of the Missing Value."@en ;
                     rdfs:isDefinedBy : ;
                     rdfs:label "Imputation Procedure"@en .


###  https://w3id.org/datamining4eepsa#IterativeValueEstimation
:IterativeValueEstimation rdf:type owl:Class ;
                          rdfs:subClassOf :ValueEstimationProcedure ;
                          <http://purl.org/ontology/bibo/status> "testing"@en ;
                          rdfs:comment "Iterative Value Estimation procedure to impute a Missing Value."@en ;
                          rdfs:isDefinedBy : ;
                          rdfs:label "Iterative Value Estimation"@en .


###  https://w3id.org/datamining4eepsa#LongMissingValueChunk
:LongMissingValueChunk rdf:type owl:Class ;
                       rdfs:subClassOf :MissingValueChunk ;
                       <http://purl.org/ontology/bibo/status> "testing"@en ;
                       rdfs:comment "A chunk of Missing Values which is considered to have a long length."@en ;
                       rdfs:isDefinedBy : ;
                       rdfs:label "Long Missing Value Chunk"@en .


###  https://w3id.org/datamining4eepsa#MAR
:MAR rdf:type owl:Class ;
     rdfs:subClassOf :MissingValue ;
     <http://purl.org/ontology/bibo/status> "testing"@en ;
     rdfs:comment "Misingness at Random (MAR): When a pattern can be identified for observation's failure."@en ;
     rdfs:isDefinedBy : ;
     rdfs:label "MAR"@en .


###  https://w3id.org/datamining4eepsa#MCAR
:MCAR rdf:type owl:Class ;
      rdfs:subClassOf :MissingValue ;
      <http://purl.org/ontology/bibo/status> "testing"@en ;
      rdfs:comment "Missingness Completely at Random (MCAR): When an observation fails randomly."@en ;
      rdfs:isDefinedBy : ;
      rdfs:label "MCAR"@en .


###  https://w3id.org/datamining4eepsa#MIV
:MIV rdf:type owl:Class ;
     rdfs:subClassOf :MNAR ;
     <http://purl.org/ontology/bibo/status> "testing"@en ;
     rdfs:comment "Misingness that depends on its value itself (MIV): When the failure of an observation depends on ints own value."@en ;
     rdfs:isDefinedBy : ;
     rdfs:label "MIV"@en .


###  https://w3id.org/datamining4eepsa#MNAR
:MNAR rdf:type owl:Class ;
      rdfs:subClassOf :MissingValue ;
      <http://purl.org/ontology/bibo/status> "testing"@en ;
      rdfs:comment "Misingness not at Random (MNAR): When an observation fails with a pattern which is unidentifiable."@en ;
      rdfs:isDefinedBy : ;
      rdfs:label "MNAR"@en .


###  https://w3id.org/datamining4eepsa#MUOV
:MUOV rdf:type owl:Class ;
      rdfs:subClassOf :MNAR ;
      <http://purl.org/ontology/bibo/status> "testing"@en ;
      rdfs:comment "Misingness that depends on unobserved variables (MUOV): When the variables that explain the cause of the observation's failure are not collected."@en ;
      rdfs:isDefinedBy : ;
      rdfs:label "MUOV"@en .


###  https://w3id.org/datamining4eepsa#MissingValue
:MissingValue rdf:type owl:Class ;
              rdfs:subClassOf <http://www.w3.org/ns/sosa/Observation> ;
              <http://purl.org/ontology/bibo/status> "stable"@en ;
              rdfs:comment "When no data is stored in an attribute of an observation."@en ;
              rdfs:isDefinedBy : ;
              rdfs:label "Missing Value"@en .


###  https://w3id.org/datamining4eepsa#MissingValueChunk
:MissingValueChunk rdf:type owl:Class ;
                   rdfs:subClassOf [ rdf:type owl:Restriction ;
                                     owl:onProperty :requiresImputationProcedure ;
                                     owl:someValuesFrom :ImputationProcedure
                                   ] ;
                   <http://purl.org/ontology/bibo/status> "testing"@en ;
                   rdfs:comment "A chunk of Missing Values."@en ;
                   rdfs:isDefinedBy : ;
                   rdfs:label "Missing Value Chunk"@en .


###  https://w3id.org/datamining4eepsa#MultipleValuesEstimation
:MultipleValuesEstimation rdf:type owl:Class ;
                          rdfs:subClassOf :ValueEstimationProcedure ;
                          <http://purl.org/ontology/bibo/status> "testing"@en ;
                          rdfs:comment "Multiple Values Estimation procedure to impute a Missing Value."@en ;
                          rdfs:isDefinedBy : ;
                          rdfs:label "Multiple Values Estimation"@en .


###  https://w3id.org/datamining4eepsa#Outlier
:Outlier rdf:type owl:Class ;
         rdfs:subClassOf <http://www.w3.org/ns/sosa/Observation> ;
         <http://purl.org/ontology/bibo/status> "stable"@en ;
         rdfs:comment "Observations that stand out and do not conform to the expected behaviour."@en ;
         rdfs:isDefinedBy : ;
         rdfs:label "Outlier"@en .


###  https://w3id.org/datamining4eepsa#OutlierCausedByBeamSpotlight
:OutlierCausedByBeamSpotlight rdf:type owl:Class ;
                              rdfs:subClassOf :OutlierCausedByDeviceLocation ;
                              <http://purl.org/ontology/bibo/status> "stable"@en ;
                              rdfs:comment "An Outlier caused by a beam spotlight. For example, an observation made by a sensing device located under a light bulb"@en ;
                              rdfs:isDefinedBy : ;
                              rdfs:label "Outlier caused by Beam Spotlight"@en .


###  https://w3id.org/datamining4eepsa#OutlierCausedByDeviceError
:OutlierCausedByDeviceError rdf:type owl:Class ;
                            rdfs:subClassOf :Outlier ,
                                            [ rdf:type owl:Restriction ;
                                              owl:onProperty :hasSolvingProcedure ;
                                              owl:someValuesFrom :ProcedureUponDevice
                                            ] ;
                            <http://purl.org/ontology/bibo/status> "stable"@en ;
                            rdfs:comment "An Outlier occurred by an error on the device itself."@en ;
                            rdfs:isDefinedBy : ;
                            rdfs:label "Outlier caused by Device Error"@en .


###  https://w3id.org/datamining4eepsa#OutlierCausedByDeviceLocation
:OutlierCausedByDeviceLocation rdf:type owl:Class ;
                               rdfs:subClassOf :Outlier ,
                                               [ rdf:type owl:Restriction ;
                                                 owl:onProperty :hasSolvingProcedure ;
                                                 owl:someValuesFrom :DeviceRelocation
                                               ] ;
                               <http://purl.org/ontology/bibo/status> "stable"@en ;
                               rdfs:comment "An Outlier occurred by the inadequate location of the device."@en ;
                               rdfs:isDefinedBy : ;
                               rdfs:label "Outlier caused by Device Location"@en .


###  https://w3id.org/datamining4eepsa#OutlierCausedByDeviceLowBattery
:OutlierCausedByDeviceLowBattery rdf:type owl:Class ;
                                 rdfs:subClassOf :OutlierCausedByDeviceError ;
                                 <http://purl.org/ontology/bibo/status> "stable"@en ;
                                 rdfs:comment "An Outlier caused by the low battery of the device."@en ;
                                 rdfs:isDefinedBy : ;
                                 rdfs:label "Outlier caused by Device Low Battery"@en .


###  https://w3id.org/datamining4eepsa#OutlierCausedByDeviceMalfunction
:OutlierCausedByDeviceMalfunction rdf:type owl:Class ;
                                  rdfs:subClassOf :OutlierCausedByDeviceError ,
                                                  [ rdf:type owl:Restriction ;
                                                    owl:onProperty :hasSolvingProcedure ;
                                                    owl:someValuesFrom :DeviceReplacement
                                                  ] ;
                                  <http://purl.org/ontology/bibo/status> "stable"@en ;
                                  rdfs:comment "An Outlier caused by a malfunction suffered by the device, which might have been transient."@en ;
                                  rdfs:isDefinedBy : ;
                                  rdfs:label "Outlier caused by Device Malfunction"@en .


###  https://w3id.org/datamining4eepsa#OutlierCausedByExternalConditions
:OutlierCausedByExternalConditions rdf:type owl:Class ;
                                   rdfs:subClassOf :OutlierCausedByDeviceLocation ;
                                   <http://purl.org/ontology/bibo/status> "testing"@en ;
                                   rdfs:comment "An Outlier caused by external factors. For example for being next to a source of radiant heat or cold such as windows and poorly insulated outside walls."@en ;
                                   rdfs:isDefinedBy : ;
                                   rdfs:label "Outlier caused by External Conditions"@en .


###  https://w3id.org/datamining4eepsa#OutlierCausedByHVAC
:OutlierCausedByHVAC rdf:type owl:Class ;
                     rdfs:subClassOf :OutlierCausedByDeviceLocation ;
                     <http://purl.org/ontology/bibo/status> "stable"@en ;
                     rdfs:comment "An Outlier caused by its device's location in a point where an activated HVAC is sending hot or cold air."@en ;
                     rdfs:isDefinedBy : ;
                     rdfs:label "Outlier caused by HVAC"@en .


###  https://w3id.org/datamining4eepsa#OutlierCausedByRain
:OutlierCausedByRain rdf:type owl:Class ;
                     rdfs:subClassOf :OutlierCausedByDeviceLocation ,
                                     [ rdf:type owl:Restriction ;
                                       owl:onProperty :hasSolvingProcedure ;
                                       owl:someValuesFrom :DeviceShelter
                                     ] ;
                     <http://purl.org/ontology/bibo/status> "stable"@en ;
                     rdfs:comment "An Outlier caused by rainfall affecting the device."@en ;
                     rdfs:isDefinedBy : ;
                     rdfs:label "Outlier caused by Rain"@en .


###  https://w3id.org/datamining4eepsa#OutlierCausedBySolarRadiation
:OutlierCausedBySolarRadiation rdf:type owl:Class ;
                               rdfs:subClassOf :OutlierCausedByDeviceLocation ,
                                               [ rdf:type owl:Restriction ;
                                                 owl:onProperty :hasSolvingProcedure ;
                                                 owl:someValuesFrom :DeviceShelter
                                               ] ;
                               <http://purl.org/ontology/bibo/status> "stable"@en ;
                               rdfs:comment "An Outlier caused by direct sunlight on the device."@en ;
                               rdfs:isDefinedBy : ;
                               rdfs:label "Outlier caused by Solar Radiation"@en .


###  https://w3id.org/datamining4eepsa#ProcedureUponDevice
:ProcedureUponDevice rdf:type owl:Class ;
                     rdfs:subClassOf <http://www.w3.org/ns/sosa/Procedure> ;
                     <http://purl.org/ontology/bibo/status> "testing"@en ;
                     rdfs:comment "Procedure that attempts to solve a problem by proceeding upon the Device."@en ;
                     rdfs:isDefinedBy : ;
                     rdfs:label "Procedure Upon Device"@en .


###  https://w3id.org/datamining4eepsa#ShortMissingValueChunk
:ShortMissingValueChunk rdf:type owl:Class ;
                        rdfs:subClassOf :MissingValueChunk ;
                        <http://purl.org/ontology/bibo/status> "testing"@en ;
                        rdfs:comment "A chunk of Missing Values which is considered to have a short length."@en ;
                        rdfs:isDefinedBy : ;
                        rdfs:label "Short Missing Value Chunk"@en .


###  https://w3id.org/datamining4eepsa#SimpleValueDrawing
:SimpleValueDrawing rdf:type owl:Class ;
                    rdfs:subClassOf :ValueDrawingProcedure ;
                    <http://purl.org/ontology/bibo/status> "testing"@en ;
                    rdfs:comment "Simple Value Drawing procedure to impute a Missing Value."@en ;
                    rdfs:isDefinedBy : ;
                    rdfs:label "Simple Value Drawing"@en .


###  https://w3id.org/datamining4eepsa#SimpleValueEstimation
:SimpleValueEstimation rdf:type owl:Class ;
                       rdfs:subClassOf :ValueEstimationProcedure ;
                       <http://purl.org/ontology/bibo/status> "testing"@en ;
                       rdfs:comment "Simple Value Estimation procedure to impute a Missing Value."@en ;
                       rdfs:isDefinedBy : ;
                       rdfs:label "Simple Value Estimation"@en .


###  https://w3id.org/datamining4eepsa#ValueDrawingProcedure
:ValueDrawingProcedure rdf:type owl:Class ;
                       rdfs:subClassOf :ImputationProcedure ;
                       <http://purl.org/ontology/bibo/status> "testing"@en ;
                       rdfs:comment "Procedure that consists in drawing a value to impute a Missing Value."@en ;
                       rdfs:isDefinedBy : ;
                       rdfs:label "Value Drawing Procedure"@en .


###  https://w3id.org/datamining4eepsa#ValueEstimationProcedure
:ValueEstimationProcedure rdf:type owl:Class ;
                          rdfs:subClassOf :ImputationProcedure ;
                          <http://purl.org/ontology/bibo/status> "testing"@en ;
                          rdfs:comment "Procedure that consists in estimating a value to impute a Missing Value."@en ;
                          rdfs:isDefinedBy : ;
                          rdfs:label "Value Estimation Procedure"@en .


###  Generated by the OWL API (version 5.1.7) https://github.com/owlcs/owlapi/
